feasability

src/MutableMap/MutableMap.dfy
@@ -5,36 +5,117 @@
 
 // RUN: %dafny /compile:0 "%s"
 
-module {:options "/functionSyntax:4"} MutableMap {
-    class MutableMap<K,V> {
-      function {:extern} content(): map<K, V>
+module {:extern "MutableMap"} {:options "/functionSyntax:4"} MutableMap {
+  class {:extern} MutableMap<K(==),V> {
+    function {:extern} content(): map<K, V>
+      reads this
 
-      constructor {:extern} ()
-        ensures this.content() == map[]
+    constructor {:extern} ()
+      ensures this.content() == map[]
+      ensures |this.content()| == 0
 
-      method {:extern} Add(k: K, v: V)
-        modifies this 
-        ensures k in content().Keys && v in content().Values
+    method {:extern} Put(k: K, v: V)
+      modifies this 
+      ensures k in this.content().Keys
+      ensures v in this.content().Values
+      ensures this.content()[k] == v
+      ensures 
+        if k !in old(this.content)() then  
+          |this.content()| == |old(this.content)()| + 1 
+        else 
+          |this.content()| == |old(this.content)()|
 
-      function {:extern} Keys(): (keys: set<K>)
-        reads this
-        ensures keys == content().Keys
+    function {:extern} Keys(): (keys: set<K>)
+      reads this
+      ensures keys == this.content().Keys
 
-      function {:extern} Values(): (values: set<V>)
-        reads this
-        ensures values == content().Values
+    function {:extern} Values(): (values: set<V>)
+      reads this
+      ensures values == this.content().Values
 
-      function {:extern} Find(k: K): (v: V)
-        reads this
-        requires k in this.Keys()
-        ensures v in content().Values
-      
-      method {:extern} Remove(k: K)
-        modifies this
-        ensures this.content().Keys == old(this.content)().Keys - {k}
+    function {:extern} Find(k: K): (v: V)
+      reads this
+      requires k in this.Keys()
+      ensures v in this.content().Values
+      ensures this.content()[k] == v
+    
+    method {:extern} Remove(k: K)
+      modifies this
+      ensures this.content().Keys == old(this.content)().Keys - {k}
+      ensures 
+        if k in old(this.content)() then 
+          && |this.content()| == |old(this.content)()| - 1 
+          && this.content().Values == old(this.content)().Values - { old(this.content)()[k] }
+        else 
+          |this.content()| == |old(this.content)()|
 
-      function {:extern} Size(): (size: int)
-        reads this
-        ensures size == |content().Values|
+    function {:extern} Size(): (size: int)
+      reads this
+      ensures size == |this.content()|
+  }
+}
+
+module {:options "/functionSyntax:4"} MutableMapFeasability refines MutableMap {
+  class MutableMap<K(==),V> ... {
+    var m: map<K,V>
+
+    function content(): map<K, V> {
+      m
     }
+
+    constructor ()
+    {
+      m := map[];
+    }
+
+    method Put(k: K, v: V) 
+    {
+      m := m[k := v];
+    }
+
+    function Keys(): (keys: set<K>)
+    {
+      m.Keys
+    }
+
+    function Values(): (values: set<V>)
+    {
+      m.Values
+    }
+
+    function Find(k: K): (v: V)
+    {
+      m[k]
+    }
+
+    method Remove(k: K)
+    {
+      m := (map k' | k' in m && k' != k :: m[k']);
+    }
+
+    function Size(): (size: int)
+    {
+      |m|
+    }
+  }
+}
+
+module Program {
+  import opened MutableMapFeasability
+
+  method Main() {
+    var m := new MutableMap<string,string>();
+    assert m.Size() == 0;
+    assert "testkey" !in m.Keys();
+    m.Put("testkey", "testvalue");
+    //assert m.Size() == 1;
+    assert "testkey" in m.Keys();
+    assert "testvalue" in m.Values();
+    assert m.Find("testkey") == "testvalue";
+    m.Remove("testkey");
+    assert "testkey" !in m.Keys();
+    m.Put("testkey", "testvalue");
+    assert "testkey" in m.Keys();
+    //assert m.Size() == 1;
+  }
 }
