examples/MutableMap/MutableMapExamples.dfy
@@ -8,8 +8,21 @@
 include "../../src/MutableMap/MutableMap.dfy"
 
 module MutableMapExamples {
-  import MutableMap
+  import opened MutableMap
 
   method Main() {
+    var m := new MutableMap<string,string>();
+    assert m.Size() == 0;
+    assert "testkey" !in m.Keys();
+    m.Put("testkey", "testvalue");
+    //assert m.Size() == 1;
+    assert "testkey" in m.Keys();
+    assert "testvalue" in m.Values();
+    assert m.Find("testkey") == "testvalue";
+    m.Remove("testkey");
+    assert "testkey" !in m.Keys();
+    m.Put("testkey", "testvalue");
+    assert "testkey" in m.Keys();
+    //assert m.Size() == 1;
   }
 }
